Lake/Build/Store.lean
@@ -27,14 +27,20 @@ abbrev BuildStore :=
 
 namespace BuildStore
 
+-- Linter reports false positives on the `v` variables below
+set_option linter.unusedVariables false
+
 /-- Derive an array of built module facets from the store. -/
 def collectModuleFacetArray (self : BuildStore)
 (facet : WfName) [DynamicType ModuleData facet α] : Array α := Id.run do
   let mut res : Array α := #[]
   for ⟨k, v⟩ in self do
-    if h : k.isModuleKey ∧ k.facet = facet then
-      let of_data := by unfold BuildData; simp [h, eq_dynamic_type]
-      res := res.push <| cast of_data v
+    match k with
+    | .moduleFacet m f =>
+      if h : f = facet then
+        have of_data := by unfold BuildData; simp [h, eq_dynamic_type]
+        res := res.push <| cast of_data v
+    | _ => pure ()
   return res
 
 /-- Derive a map of module names to built facets from the store. -/
@@ -42,27 +48,41 @@ def collectModuleFacetMap (self : BuildStore)
 (facet : WfName) [DynamicType ModuleData facet α] : NameMap α := Id.run do
   let mut res := Lean.mkNameMap α
   for ⟨k, v⟩ in self do
-    if h : k.isModuleKey ∧ k.facet = facet then
-      let of_data := by simp [isModuleKey_data h.1, h.2, eq_dynamic_type]
-      res := res.insert (k.module h.1) <| cast of_data v
+    match k with
+    | .moduleFacet m f =>
+      if h : f = facet then
+        have of_data := by unfold BuildData; simp [h, eq_dynamic_type]
+        res := res.insert m <| cast of_data v
+    | _ => pure ()
   return res
 
-/-- Derive an array of built module facets from the store. -/
+/-- Derive an array of built package facets from the store. -/
 def collectPackageFacetArray (self : BuildStore)
 (facet : WfName) [DynamicType PackageData facet α] : Array α := Id.run do
   let mut res : Array α := #[]
   for ⟨k, v⟩ in self do
-    if h : k.isPackageKey ∧ k.facet = facet then
-      let of_data := by simp [isPackageKey_data h.1, h.2, eq_dynamic_type]
-      res := res.push <| cast of_data v
+    match k with
+    | .packageFacet _ f =>
+      if h : f = facet then
+        have of_data := by unfold BuildData; simp [h, eq_dynamic_type]
+        res := res.push <| cast of_data v
+    | _ => pure ()
+  return res
+
+/-- Derive an array of built target facets from the store. -/
+def collectTargetFacetArray (self : BuildStore)
+(facet : WfName) [DynamicType TargetData facet α] : Array α := Id.run do
+  let mut res : Array α := #[]
+  for ⟨k, v⟩ in self do
+    match k with
+    | .targetFacet _ _ f =>
+      if h : f = facet then
+        have of_data := by unfold BuildData; simp [h, eq_dynamic_type]
+        res := res.push <| cast of_data v
+    | _ => pure ()
   return res
 
 /-- Derive an array of built external shared libraries from the store. -/
 def collectSharedExternLibs (self : BuildStore)
-[DynamicType TargetData &`externLib.shared α] : Array α := Id.run do
-  let mut res : Array α := #[]
-  for ⟨k, v⟩ in self do
-    if h : k.isTargetKey ∧ k.facet = &`externLib.shared then
-      let of_data := by simp [isTargetKey_data h.1, h.2, eq_dynamic_type]
-      res := res.push <| cast of_data v
-  return res
+[DynamicType TargetData &`externLib.shared α] : Array α :=
+  self.collectTargetFacetArray &`externLib.shared
